LocalLang/SemanticsExamples.lean
@@ -1,89 +1,95 @@
 import LocalLang.Semantics
-import LocalLang.SemanticsLemmas
-import LocalLang.Ctx
-import Mathlib.Data.List.Sigma
-import Std.Data.HashMap.Basic
-import Std.Data.HashMap.Lemmas
 
-instance : Add Expr where
-  add := .binOp .add
+def f_body : Expr := .binOp .add
+  (
+    .funCall "g" [
+      .binOp .add (.var "x") (.const 1)
+    ]
+  )
+  (
+    .var "x"
+  )
+def f : Function := ⟨
+  "f",
+  ["x"],
+  f_body
+⟩
+def g : Function := ⟨
+  "g",
+  ["x"],
+  .var "x"
+⟩
 
-instance : Coe String Expr where
-  coe := .var
+def f_body₂ : Expr := .binOp .add
+  (.letIn "x" (.binOp .add (.var "x") (.const 1)) (.var "x"))
+  (.var "x")
+def f_body₃ : Expr := .binOp .add
+  (.letIn "x" (.binOp .add (.const 0) (.const 1)) (.var "x"))
+  (.var "x")
+def f_body₄ : Expr := .binOp .add
+  (.letIn "x" (.const 1) (.var "x"))
+  (.var "x")
+def f_body₅ : Expr := .binOp .add
+  (.letIn "x" (.const 1) (.const 1))
+  (.var "x")
+def f_body₆ : Expr := .binOp .add (.const 1) (.var "x")
+def f_body₇ : Expr := .binOp .add (.const 1) (.const 0)
+def f_body₈ : Expr := .const 1
+def e₁ : Expr := .funCall "f" [.const 0]
+def e₂ : Expr := .letIn "x" (.const 0) f_body
+def e₃ : Expr := .letIn "x" (.const 0) f_body₂
+def e₄ : Expr := .letIn "x" (.const 0) f_body₃
+def e₅ : Expr := .letIn "x" (.const 0) f_body₄
+def e₆ : Expr := .letIn "x" (.const 0) f_body₅
+def e₇ : Expr := .letIn "x" (.const 0) f_body₆
+def e₈ : Expr := .letIn "x" (.const 0) f_body₇
+def e₉ : Expr := .letIn "x" (.const 0) f_body₈
+def e₁₀ : Expr := .const 1
+def step₁ : SmallStep [f, g] ∅ e₁ e₂ := by
+  let almost := @SmallStep.fun_step [f, g] ∅ "f" ["x"] f_body [.const 0] (by simp [f]) (by simp)
+  simp [f, letin_chain] at almost
+  rw [← f, ← e₁, ← e₂] at almost
+  assumption
+def step₂ : SmallStep [f, g] ∅ e₂ e₃ := by
+  let a : SmallStep [f, g] (.ofList [("x", 0)])
+    (.funCall "g" [.binOp .add (.var "x") (.const 1)])
+    (.letIn "x" (.binOp .add (.var "x") (.const 1)) (.var "x")) :=
+    @SmallStep.fun_step [f, g] (.ofList [("x", 0)]) "g" ["x"] g.body
+      [.binOp .add (.var "x") (.const 1)] (by simp [f, g]) (by simp)
+  let b : SmallStep [f, g] (.ofList [("x", 0)]) f_body f_body₂ :=
+    .ctx_step (.bin_op_lhs .hole .add (.var "x")) a
+  exact .letin_cong b
+def step₃ : SmallStep [f, g] ∅ e₃ e₄ := by
+  let a : SmallStep [f, g] (.ofList [("x", 0)]) f_body₂ f_body₃ :=
+    .ctx_step (.bin_op_lhs
+      (.letin "x" (.bin_op_lhs .hole .add (.const 1)) (.var "x"))
+      .add
+      (.var "x")
+    ) (.var_step (by simp))
+  exact .letin_cong a
+def step₄ : SmallStep [f, g] ∅ e₄ e₅ := by
+  let a : SmallStep [f, g] (.ofList [("x", 0)]) f_body₃ f_body₄ :=
+    .ctx_step (.bin_op_lhs
+      (.letin "x" .hole (.var "x"))
+      .add
+      (.var "x")
+    ) .bin_op_step
+  exact .letin_cong a
+def step₅ : SmallStep [f, g] ∅ e₅ e₆ := by
+  let a : SmallStep [f, g] (.ofList [("x", 0)])
+    (.letIn "x" (.const 1) (.var "x"))
+    (.letIn "x" (.const 1) (.const 1)) :=
+    .letin_cong (.var_step (by simp))
+  let b := SmallStep.ctx_step (.bin_op_lhs .hole .add (.var "x")) a
+  exact .letin_cong b
+def step₆ : SmallStep [f, g] ∅ e₆ e₇ :=
+  .letin_cong <| SmallStep.ctx_step (.bin_op_lhs .hole .add (.var "x")) .letin_const_step
+def step₇ : SmallStep [f, g] ∅ e₇ e₈ :=
+  .letin_cong <| .ctx_step (.bin_op_rhs 1 .add .hole) (.var_step (by simp))
+def step₈ : SmallStep [f, g] ∅ e₈ e₉ :=
+  .letin_cong <| .bin_op_step
+def step₉ : SmallStep [f, g] ∅ e₉ e₁₀ :=
+  .letin_const_step
 
-instance : OfNat Expr n where
-  ofNat := .const n
-
-abbrev f_body : Expr := (.funCall "g" [ "x" + 1 ]) + "x"
-abbrev f : Function := {
-  parameters := ["x"],
-  body := f_body
-}
-abbrev g : Function := {
-  parameters := ["x"],
-  body := "x"
-}
-
-abbrev defs := Std.HashMap.ofList [("f", f), ("g", g)]
-
-@[simp] lemma defs_f : defs["f"] = f := by
-  apply (Std.HashMap.getElem_ofList_of_mem (k := "f")) <;> simp
-@[simp] lemma defs_g : defs["g"] = g := by
-  apply (Std.HashMap.getElem_ofList_of_mem (k := "g")) <;> simp
-
-lemma f_steps
-  : SmallSteps defs (Std.HashMap.ofList [("x", 0)])
-      (Expr.funCall "g" ["x" + 1] + Expr.var "x") 1 := by
-  let locals := Std.HashMap.ofList [("x", 0)]
-  calc
-    SmallSteps defs locals _ (1 + "x") := by
-      apply (SmallSteps.with_ctx (.binOpLhs .hole .add "x") rfl rfl)
-      simp only [Ctx.updateEnv]
-      calc
-        SmallStep defs locals _ (.letIn "x" ("x" + 1) "x") := by
-          apply SmallStep.hole_step
-          apply (HeadSmallStep.fun_step ?_ rfl) <;> try rw [defs_g]
-          · simp
-          · rfl
-          · simp
-        SmallSteps defs locals _ (.letIn "x" 1 "x") := by
-          apply (SmallSteps.with_ctx (.letInExpr "x" .hole "x") rfl rfl)
-          calc
-            SmallStep defs locals _ ((0 : Expr) + 1) := by
-              apply (SmallStep.ctx_step (.binOpLhs .hole .add 1) rfl rfl)
-              constructor
-              simp [locals]
-            SmallStep defs locals _ _ := by
-              apply SmallStep.hole_step
-              constructor
-              rfl
-        SmallStep defs locals _ (.letIn "x" 1 1) := by
-          apply (SmallStep.ctx_step (.letInBody "x" 1 .hole) rfl rfl)
-          constructor
-          simp
-        SmallStep defs locals _ 1 := by
-          apply SmallStep.hole_step
-          constructor
-    SmallStep defs locals _ ((1 : Expr) + 0) := by
-      apply (SmallStep.ctx_step (.binOpRhs 1 .add .hole) rfl rfl)
-      constructor
-      simp [locals]
-    SmallStep defs locals _ _ := by
-      apply SmallStep.hole_step
-      constructor
-      rfl
-
-example : SmallSteps defs ∅ (.funCall "f" [0]) 1 := by
-  calc
-    SmallStep defs ∅ _ (.letIn "x" 0 f_body) := by
-      apply SmallStep.hole_step
-      apply (HeadSmallStep.fun_step ?_ rfl) <;> try rw [defs_f]
-      · simp
-      · rfl
-      · simp
-    SmallSteps defs ∅ _ (.letIn "x" 0 1) := by
-      apply (SmallSteps.with_ctx (.letInBody "x" 0 .hole) rfl rfl)
-      exact f_steps
-    SmallStep defs ∅ _ _ := by
-      apply SmallStep.hole_step
-      constructor
+def steps : SmallSteps [f, g] ∅ e₁ (.const 1) := .cons step₁ <| .cons step₂ <| .cons step₃ <|
+  .cons step₄ <| .cons step₅ <| .cons step₆ <| .cons step₇ <| .cons step₈ <| .cons step₉ <| .trivial
